WP rules - lea jmp and subseg

theories/rules/rules_Lea.v
@@ -14,60 +14,61 @@ Section cap_lang_rules.
   Implicit Types r : RegName.
   Implicit Types v : cap_lang.val.
   Implicit Types w : Word.
-  Implicit Types reg : gmap RegName Word.
+  Implicit Types reg : gmap (CoreN * RegName) Word.
   Implicit Types ms : gmap Addr Word.
 
-  Inductive Lea_failure (regs: Reg) (r1: RegName) (rv: Z + RegName) :=
+  Inductive Lea_failure (i: CoreN) (regs: Reg) (r1: RegName) (rv: Z + RegName) :=
   | Lea_fail_rv_nonconst :
-     z_of_argument regs rv = None ->
-     Lea_failure regs r1 rv
+     z_of_argument regs i rv = None ->
+     Lea_failure i regs r1 rv
   | Lea_fail_p_E : forall p b e a,
-     regs !! r1 = Some (WCap p b e a) ->
+     regs !! (i, r1) = Some (WCap p b e a) ->
      p = E ->
-     Lea_failure regs r1 rv
+     Lea_failure i regs r1 rv
   | Lea_fail_r1_noncap : forall n,
-     regs !! r1 = Some (WInt n) ->
-     Lea_failure regs r1 rv
+     regs !! (i, r1) = Some (WInt n) ->
+     Lea_failure i regs r1 rv
   | Lea_fail_overflow : forall p b e a z,
-     regs !! r1 = Some (WCap p b e a) ->
-     z_of_argument regs rv = Some z ->
+     regs !! (i, r1) = Some (WCap p b e a) ->
+     z_of_argument regs i rv = Some z ->
      (a + z)%a = None ->
-     Lea_failure regs r1 rv
+     Lea_failure i regs r1 rv
   | Lea_fail_overflow_PC : forall p b e a z a',
-     regs !! r1 = Some (WCap p b e a) ->
-     z_of_argument regs rv = Some z ->
+     regs !! (i, r1) = Some (WCap p b e a) ->
+     z_of_argument regs i rv = Some z ->
      (a + z)%a = Some a' ->
-     incrementPC (<[ r1 := WCap p b e a' ]> regs) = None ->
-     Lea_failure regs r1 rv
+     incrementPC (<[ (i, r1) := WCap p b e a' ]> regs) i = None ->
+     Lea_failure i regs r1 rv
    .
 
   Inductive Lea_spec
+    (i : CoreN)
     (regs: Reg) (r1: RegName) (rv: Z + RegName)
     (regs': Reg) : cap_lang.val → Prop
   :=
   | Lea_spec_success : forall p b e a z a',
-    regs !! r1 = Some (WCap p b e a) ->
+    regs !! (i, r1) = Some (WCap p b e a) ->
     p ≠ E ->
-    z_of_argument regs rv = Some z ->
+    z_of_argument regs i rv = Some z ->
     (a + z)%a = Some a' ->
     incrementPC
-      (<[ r1 := WCap p b e a' ]> regs) = Some regs' ->
-    Lea_spec regs r1 rv regs' NextIV
+      (<[ (i, r1) := WCap p b e a' ]> regs) i = Some regs' ->
+    Lea_spec i regs r1 rv regs' (i, NextIV)
 
   | Lea_spec_failure :
-    Lea_failure regs r1 rv ->
-    Lea_spec regs r1 rv regs' FailedV.
+    Lea_failure i regs r1 rv ->
+    Lea_spec i regs r1 rv regs' (i, FailedV).
 
-   Lemma wp_lea Ep pc_p pc_b pc_e pc_a r1 w arg (regs: Reg) :
+   Lemma wp_lea Ep i pc_p pc_b pc_e pc_a r1 w arg (regs: Reg) :
      decodeInstrW w = Lea r1 arg →
      isCorrectPC (WCap pc_p pc_b pc_e pc_a) →
-     regs !! PC = Some (WCap pc_p pc_b pc_e pc_a) →
-     regs_of (Lea r1 arg) ⊆ dom _ regs →
+     regs !! (i, PC) = Some (WCap pc_p pc_b pc_e pc_a) →
+     regs_of_core (Lea r1 arg) i ⊆ dom _ regs →
      {{{ ▷ pc_a ↦ₐ w ∗
          ▷ [∗ map] k↦y ∈ regs, k ↦ᵣ y }}}
-       Instr Executable @ Ep
+       (i, Instr Executable) @ Ep
      {{{ regs' retv, RET retv;
-         ⌜ Lea_spec regs r1 arg regs' retv ⌝ ∗
+         ⌜ Lea_spec i regs r1 arg regs' retv ⌝ ∗
          pc_a ↦ₐ w ∗
          [∗ map] k↦y ∈ regs', k ↦ᵣ y }}}.
    Proof.
@@ -81,19 +82,19 @@ Section cap_lang_rules.
      iModIntro. iSplitR. by iPureIntro; apply normal_always_head_reducible.
      iNext. iIntros (e2 σ2 efs Hpstep).
      apply prim_step_exec_inv in Hpstep as (-> & -> & (c & -> & Hstep)).
-     iSplitR; auto. eapply step_exec_inv in Hstep; eauto.
+     iSplitR; auto. eapply core_step_exec_inv in Hstep; eauto.
      unfold exec in Hstep; simpl in Hstep.
 
-     specialize (indom_regs_incl _ _ _ Dregs Hregs) as Hri. unfold regs_of in Hri.
+     specialize (indom_regs_incl _ _ _ Dregs Hregs) as Hri. unfold regs_of_core in Hri.
 
-     feed destruct (Hri r1) as [r1v [Hr'1 Hr1]]. by set_solver+.
+     feed destruct (Hri i r1) as [r1v [Hr'1 Hr1]]. by set_solver+.
      rewrite Hr1 in Hstep.
 
-     destruct (z_of_argument regs arg) as [ argz |] eqn:Harg;
+     destruct (z_of_argument regs i arg) as [ argz |] eqn:Harg;
        pose proof Harg as Harg'; cycle 1.
      { (* Failure: argument is not a constant (z_of_argument regs arg = None) *)
        unfold z_of_argument in Harg, Hstep. destruct arg as [| r0]; [ congruence |].
-       feed destruct (Hri r0) as [r0v [Hr'0 Hr0]].
+       feed destruct (Hri i r0) as [r0v [Hr'0 Hr0]].
        { unfold regs_of_argument. set_solver+. }
        rewrite Hr0 Hr'0 in Harg Hstep.
        destruct r0v; [ congruence |].
@@ -120,20 +121,20 @@ Section cap_lang_rules.
          iFailWP "Hφ" Lea_fail_overflow. }
 
      rewrite /update_reg /= in Hstep.
-     destruct (incrementPC (<[ r1 := WCap p b e a' ]> regs)) as [ regs' |] eqn:Hregs';
+     destruct (incrementPC (<[ (i, r1) := WCap p b e a' ]> regs) i) as [ regs' |] eqn:Hregs';
        pose proof Hregs' as Hregs'2; cycle 1.
      { (* Failure: incrementing PC overflows *)
-       assert (incrementPC (<[ r1 := WCap p b e a' ]> r) = None) as HH.
+       assert (incrementPC (<[ (i , r1) := WCap p b e a' ]> r) i = None) as HH.
        { eapply incrementPC_overflow_mono; first eapply Hregs'.
          by rewrite lookup_insert_is_Some'; eauto.
          by apply insert_mono; eauto. }
-       apply (incrementPC_fail_updatePC _ m) in HH. rewrite HH in Hstep.
+       apply (incrementPC_fail_updatePC _ i m) in HH. rewrite HH in Hstep.
        assert (c = Failed ∧ σ2 = (r, m)) as (-> & ->)
            by (destruct p; inversion Hstep; auto).
        iFailWP "Hφ" Lea_fail_overflow_PC. }
 
      (* Success *)
-     eapply (incrementPC_success_updatePC _ m) in Hregs'
+     eapply (incrementPC_success_updatePC _ i m) in Hregs'
        as (p' & g' & b' & e' & a'' & a_pc' & HPC'' & HuPC & ->).
      eapply updatePC_success_incl in HuPC. 2: by eapply insert_mono; eauto.
      rewrite HuPC in Hstep; clear HuPC.
@@ -142,145 +143,153 @@ Section cap_lang_rules.
      simplify_pair_eq.
 
      iFrame.
-     iMod ((gen_heap_update_inSepM _ _ r1) with "Hr Hmap") as "[Hr Hmap]"; eauto.
-     iMod ((gen_heap_update_inSepM _ _ PC) with "Hr Hmap") as "[Hr Hmap]"; eauto.
+     iMod ((gen_heap_update_inSepM _ _ (i, r1)) with "Hr Hmap") as "[Hr Hmap]"; eauto.
+     iMod ((gen_heap_update_inSepM _ _ (i, PC)) with "Hr Hmap") as "[Hr Hmap]"; eauto.
      iFrame. iModIntro. iApply "Hφ". iFrame. iPureIntro.
      eapply Lea_spec_success; eauto.
 
      Unshelve. all: auto.
    Qed.
 
-   Lemma wp_lea_success_reg_PC Ep pc_p pc_b pc_e pc_a pc_a' w rv z a' :
+   Lemma wp_lea_success_reg_PC Ep i pc_p pc_b pc_e pc_a pc_a' w rv z a' :
      decodeInstrW w = Lea PC (inr rv) →
      isCorrectPC (WCap pc_p pc_b pc_e pc_a) →
      (a' + 1)%a = Some pc_a' →
      (pc_a + z)%a = Some a' →
      pc_p ≠ E →
 
-     {{{ ▷ PC ↦ᵣ WCap pc_p pc_b pc_e pc_a
+     {{{ ▷ (i, PC) ↦ᵣ WCap pc_p pc_b pc_e pc_a
            ∗ ▷ pc_a ↦ₐ w
-           ∗ ▷ rv ↦ᵣ WInt z }}}
-       Instr Executable @ Ep
-       {{{ RET NextIV;
-           PC ↦ᵣ WCap pc_p pc_b pc_e pc_a'
+           ∗ ▷ (i, rv) ↦ᵣ WInt z }}}
+       (i, Instr Executable) @ Ep
+       {{{ RET (i, NextIV);
+           (i, PC) ↦ᵣ WCap pc_p pc_b pc_e pc_a'
               ∗ pc_a ↦ₐ w
-              ∗ rv ↦ᵣ WInt z }}}.
+              ∗ (i, rv) ↦ᵣ WInt z }}}.
    Proof.
      iIntros (Hinstr Hvpc Hpca' Ha' Hnep φ) "(>HPC & >Hpc_a & >Hrv) Hφ".
      iDestruct (map_of_regs_2 with "HPC Hrv") as "[Hmap %]".
-     iApply (wp_lea with "[$Hmap Hpc_a]"); eauto; simplify_map_eq; eauto.
-     by rewrite !dom_insert; set_solver+.
+     iApply (wp_lea with "[$Hmap Hpc_a]"); eauto
+     ; simplify_map_eq by simplify_pair_eq; eauto.
+     { rewrite !dom_insert /regs_of_core /regs_of /regs_of_argument
+       ; set_solver+. }
      iNext. iIntros (regs' retv) "(#Hspec & Hpc_a & Hmap)".
      iDestruct "Hspec" as %Hspec.
 
      destruct Hspec as [ | * Hfail ].
      { (* Success *)
-       iApply "Hφ". iFrame. incrementPC_inv; simplify_map_eq.
-       rewrite !insert_insert. (* TODO: add to simplify_map_eq via simpl_map? *)
+       iApply "Hφ". iFrame. incrementPC_inv; simplify_map_eq by simplify_pair_eq.
+       rewrite !insert_insert. (* TODO: add to simplify_map_eq by simplify_pair_eq via simpl_map? *)
        iApply (regs_of_map_2 with "Hmap"); eauto. }
      { (* Failure (contradiction) *)
-       destruct Hfail; try incrementPC_inv; simplify_map_eq; eauto. congruence.
+       destruct Hfail; try incrementPC_inv; simplify_map_eq by simplify_pair_eq; eauto. congruence.
      }
    Qed.
 
-   Lemma wp_lea_success_reg Ep pc_p pc_b pc_e pc_a pc_a' w r1 rv p b e a z a' :
+   Lemma wp_lea_success_reg Ep i pc_p pc_b pc_e pc_a pc_a' w r1 rv p b e a z a' :
      decodeInstrW w = Lea r1 (inr rv) →
      isCorrectPC (WCap pc_p pc_b pc_e pc_a) →
      (pc_a + 1)%a = Some pc_a' →
      (a + z)%a = Some a' →
      p ≠ E →
      
-     {{{ ▷ PC ↦ᵣ WCap pc_p pc_b pc_e pc_a
+     {{{ ▷ (i, PC) ↦ᵣ WCap pc_p pc_b pc_e pc_a
            ∗ ▷ pc_a ↦ₐ w
-           ∗ ▷ r1 ↦ᵣ WCap p b e a
-           ∗ ▷ rv ↦ᵣ WInt z }}}
-       Instr Executable @ Ep
-       {{{ RET NextIV;
-           PC ↦ᵣ WCap pc_p pc_b pc_e pc_a'
+           ∗ ▷ (i, r1) ↦ᵣ WCap p b e a
+           ∗ ▷ (i, rv) ↦ᵣ WInt z }}}
+       (i, Instr Executable) @ Ep
+       {{{ RET (i, NextIV);
+           (i, PC) ↦ᵣ WCap pc_p pc_b pc_e pc_a'
               ∗ pc_a ↦ₐ w
-              ∗ rv ↦ᵣ WInt z
-              ∗ r1 ↦ᵣ WCap p b e a' }}}.
+              ∗ (i, rv) ↦ᵣ WInt z
+              ∗ (i, r1) ↦ᵣ WCap p b e a' }}}.
    Proof.
      iIntros (Hinstr Hvpc Hpca' Ha' Hnep ϕ) "(>HPC & >Hpc_a & >Hr1 & >Hrv) Hφ".
      iDestruct (map_of_regs_3 with "HPC Hrv Hr1") as "[Hmap (%&%&%)]".
-     iApply (wp_lea with "[$Hmap Hpc_a]"); eauto; simplify_map_eq; eauto.
-     by rewrite !dom_insert; set_solver+.
+     iApply (wp_lea with "[$Hmap Hpc_a]"); eauto; simplify_map_eq by simplify_pair_eq; eauto.
+     { rewrite !dom_insert /regs_of_core /regs_of /regs_of_argument
+       ; set_solver+. }
      iNext. iIntros (regs' retv) "(#Hspec & Hpc_a & Hmap)".
      iDestruct "Hspec" as %Hspec.
 
      destruct Hspec as [| * Hfail ].
      { (* Success *)
-       iApply "Hφ". iFrame. incrementPC_inv; simplify_map_eq.
+       iApply "Hφ". iFrame. incrementPC_inv; simplify_map_eq by simplify_pair_eq.
        (* FIXME: tedious *)
-       rewrite (insert_commute _ PC r1) // insert_insert.
-       rewrite (insert_commute _ r1 PC) // (insert_commute _ r1 rv) // insert_insert.
+       rewrite (insert_commute _ (i, PC) (i, r1)) ; simplify_pair_eq.
+       rewrite insert_insert (insert_commute _ (i, r1) (i, PC)); simplify_pair_eq.
+       rewrite (insert_commute _ (i, r1) (i, rv)); simplify_pair_eq.
+       rewrite insert_insert.
        iApply (regs_of_map_3 with "Hmap"); eauto. }
      { (* Failure (contradiction) *)
-       destruct Hfail; try incrementPC_inv; simplify_map_eq; eauto. congruence.
+       destruct Hfail; try incrementPC_inv; simplify_map_eq by simplify_pair_eq; eauto. congruence.
      }
    Qed.
 
-   Lemma wp_lea_success_z_PC Ep pc_p pc_b pc_e pc_a pc_a' w z a' :
+   Lemma wp_lea_success_z_PC Ep i pc_p pc_b pc_e pc_a pc_a' w z a' :
      decodeInstrW w = Lea PC (inl z) →
      isCorrectPC (WCap pc_p pc_b pc_e pc_a) →
      (a' + 1)%a = Some pc_a' →
      (pc_a + z)%a = Some a' →
      pc_p ≠ E →
 
-     {{{ ▷ PC ↦ᵣ WCap pc_p pc_b pc_e pc_a
+     {{{ ▷ (i, PC) ↦ᵣ WCap pc_p pc_b pc_e pc_a
            ∗ ▷ pc_a ↦ₐ w }}}
-       Instr Executable @ Ep
-     {{{ RET NextIV;
-         PC ↦ᵣ WCap pc_p pc_b pc_e pc_a'
+       (i, Instr Executable) @ Ep
+     {{{ RET (i, NextIV);
+         (i, PC) ↦ᵣ WCap pc_p pc_b pc_e pc_a'
             ∗ pc_a ↦ₐ w }}}.
    Proof.
      iIntros (Hinstr Hvpc Hpca' Ha' Hnep ϕ) "(>HPC & >Hpc_a) Hφ".
      iDestruct (map_of_regs_1 with "HPC") as "Hmap".
-     iApply (wp_lea with "[$Hmap Hpc_a]"); eauto; simplify_map_eq; eauto.
+     iApply (wp_lea with "[$Hmap Hpc_a]"); eauto; simplify_map_eq by simplify_pair_eq; eauto.
      by rewrite !dom_insert; set_solver+.
      iNext. iIntros (regs' retv) "(#Hspec & Hpc_a & Hmap)".
      iDestruct "Hspec" as %Hspec.
 
      destruct Hspec as [ | * Hfail ].
      { (* Success *)
-       iApply "Hφ". iFrame. incrementPC_inv; simplify_map_eq.
+       iApply "Hφ". iFrame. incrementPC_inv; simplify_map_eq by simplify_pair_eq.
        rewrite !insert_insert. iApply (regs_of_map_1 with "Hmap"); eauto. }
      { (* Failure (contradiction) *)
-       destruct Hfail; try incrementPC_inv; simplify_map_eq; eauto. congruence.
+       destruct Hfail; try incrementPC_inv; simplify_map_eq by simplify_pair_eq; eauto. congruence.
      }
    Qed.
 
-   Lemma wp_lea_success_z Ep pc_p pc_b pc_e pc_a pc_a' w r1 p b e a z a' :
+   Lemma wp_lea_success_z Ep i pc_p pc_b pc_e pc_a pc_a' w r1 p b e a z a' :
      decodeInstrW w = Lea r1 (inl z) →
      isCorrectPC (WCap pc_p pc_b pc_e pc_a) →
      (pc_a + 1)%a = Some pc_a' →
      (a + z)%a = Some a' →
      p ≠ E →
 
-     {{{ ▷ PC ↦ᵣ WCap pc_p pc_b pc_e pc_a
+     {{{ ▷ (i, PC) ↦ᵣ WCap pc_p pc_b pc_e pc_a
            ∗ ▷ pc_a ↦ₐ w
-           ∗ ▷ r1 ↦ᵣ WCap p b e a }}}
-       Instr Executable @ Ep
-     {{{ RET NextIV;
-         PC ↦ᵣ WCap pc_p pc_b pc_e pc_a'
+           ∗ ▷ (i, r1) ↦ᵣ WCap p b e a }}}
+       (i, Instr Executable) @ Ep
+     {{{ RET (i, NextIV);
+         (i, PC) ↦ᵣ WCap pc_p pc_b pc_e pc_a'
             ∗ pc_a ↦ₐ w
-            ∗ r1 ↦ᵣ WCap p b e a' }}}.
+            ∗ (i, r1) ↦ᵣ WCap p b e a' }}}.
    Proof.
      iIntros (Hinstr Hvpc Hpca' Ha' Hnep ϕ) "(>HPC & >Hpc_a & >Hr1) Hφ".
      iDestruct (map_of_regs_2 with "HPC Hr1") as "[Hmap %]".
-     iApply (wp_lea with "[$Hmap Hpc_a]"); eauto; simplify_map_eq; eauto.
+     iApply (wp_lea with "[$Hmap Hpc_a]"); eauto; simplify_map_eq by simplify_pair_eq; eauto.
      by rewrite !dom_insert; set_solver+.
      iNext. iIntros (regs' retv) "(#Hspec & Hpc_a & Hmap)".
      iDestruct "Hspec" as %Hspec.
 
      destruct Hspec as [ | * Hfail ].
      { (* Success *)
-       iApply "Hφ". iFrame. incrementPC_inv; simplify_map_eq.
+       iApply "Hφ". iFrame. incrementPC_inv; simplify_map_eq by simplify_pair_eq.
        (* FIXME: tedious *)
-       rewrite insert_commute // insert_insert insert_commute // insert_insert.
+       rewrite (insert_commute _ (i, PC) (i, r1)) ; simplify_pair_eq
+       ; rewrite insert_insert.
+       rewrite (insert_commute _ (i, r1) (i, PC)) ; simplify_pair_eq
+       ; rewrite insert_insert.
        iDestruct (regs_of_map_2 with "Hmap") as "[? ?]"; eauto. iFrame. }
      { (* Failure (contradiction) *)
-       destruct Hfail; try incrementPC_inv; simplify_map_eq; eauto. congruence.
+       destruct Hfail; try incrementPC_inv; simplify_map_eq by simplify_pair_eq; eauto. congruence.
      }
    Qed.
 
