theories/rules/rules_Subseg.v
@@ -13,63 +13,63 @@ Section cap_lang_rules.
   Implicit Types r : RegName.
   Implicit Types v : cap_lang.val. 
   Implicit Types w : Word.
-  Implicit Types reg : gmap RegName Word.
-  Implicit Types ms : gmap Addr Word. 
+  Implicit Types reg : gmap (CoreN * RegName) Word.
+  Implicit Types ms : gmap Addr Word.
 
-  Inductive Subseg_failure  (regs: Reg) (dst: RegName) (src1 src2: Z + RegName) : Reg → Prop :=
+  Inductive Subseg_failure (i: CoreN) (regs: Reg) (dst: RegName) (src1 src2: Z + RegName) : Reg → Prop :=
   | Subseg_fail_dst_noncap z :
-      regs !! dst = Some (WInt z) →
-      Subseg_failure regs dst src1 src2 regs
+      regs !! (i, dst) = Some (WInt z) →
+      Subseg_failure i regs dst src1 src2 regs
   | Subseg_fail_pE p b e a :
-      regs !! dst = Some (WCap p b e a) →
+      regs !! (i, dst) = Some (WCap p b e a) →
       p = E →
-      Subseg_failure regs dst src1 src2 regs
+      Subseg_failure i regs dst src1 src2 regs
   | Subseg_fail_src1_nonaddr :
-      addr_of_argument regs src1 = None →
-      Subseg_failure regs dst src1 src2 regs
+      addr_of_argument regs i src1 = None →
+      Subseg_failure i regs dst src1 src2 regs
   | Subseg_fail_src2_nonaddr :
-      addr_of_argument regs src2 = None →
-      Subseg_failure regs dst src1 src2 regs
+      addr_of_argument regs i src2 = None →
+      Subseg_failure i regs dst src1 src2 regs
   | Subseg_fail_not_iswithin p b e a a1 a2 :
-      regs !! dst = Some (WCap p b e a) →
-      addr_of_argument regs src1 = Some a1 →
-      addr_of_argument regs src2 = Some a2 →
+      regs !! (i, dst) = Some (WCap p b e a) →
+      addr_of_argument regs i src1 = Some a1 →
+      addr_of_argument regs i src2 = Some a2 →
       isWithin a1 a2 b e = false →
-      Subseg_failure regs dst src1 src2 regs
+      Subseg_failure i regs dst src1 src2 regs
   | Subseg_fail_incrPC p b e a a1 a2 :
-      regs !! dst = Some (WCap p b e a) →
+      regs !! (i, dst) = Some (WCap p b e a) →
       p <> E →
-      addr_of_argument regs src1 = Some a1 →
-      addr_of_argument regs src2 = Some a2 →
+      addr_of_argument regs i src1 = Some a1 →
+      addr_of_argument regs i src2 = Some a2 →
       isWithin a1 a2 b e = true →
-      incrementPC (<[ dst := WCap p a1 a2 a ]> regs) = None →
-      Subseg_failure regs dst src1 src2 regs.
+      incrementPC (<[ (i, dst) := WCap p a1 a2 a ]> regs) i = None →
+      Subseg_failure i regs dst src1 src2 regs.
 
-  Inductive Subseg_spec (regs: Reg) (dst: RegName) (src1 src2: Z + RegName) (regs': Reg): cap_lang.val -> Prop :=
+  Inductive Subseg_spec (i : CoreN)(regs: Reg) (dst: RegName) (src1 src2: Z + RegName) (regs': Reg): cap_lang.val -> Prop :=
   | Subseg_spec_success p b e a a1 a2:
-      regs !! dst = Some (WCap p b e a) ->
+      regs !! (i, dst) = Some (WCap p b e a) ->
       p <> E ->
-      addr_of_argument regs src1 = Some a1 ->
-      addr_of_argument regs src2 = Some a2 ->
+      addr_of_argument regs i src1 = Some a1 ->
+      addr_of_argument regs i src2 = Some a2 ->
       isWithin a1 a2 b e = true ->
-      incrementPC (<[ dst := WCap p a1 a2 a ]> regs) = Some regs' ->
-      Subseg_spec regs dst src1 src2 regs' NextIV
+      incrementPC (<[ (i, dst) := WCap p a1 a2 a ]> regs) i = Some regs' ->
+      Subseg_spec i regs dst src1 src2 regs' (i, NextIV)
   | Subseg_spec_failure :
-      Subseg_failure regs dst src1 src2 regs' →
-      Subseg_spec regs dst src1 src2 regs' FailedV.
+      Subseg_failure i regs dst src1 src2 regs' →
+      Subseg_spec i regs dst src1 src2 regs' (i, FailedV).
 
   
-  Lemma wp_Subseg Ep pc_p pc_b pc_e pc_a w dst src1 src2 regs :
+  Lemma wp_Subseg Ep i pc_p pc_b pc_e pc_a w dst src1 src2 regs :
     decodeInstrW w = Subseg dst src1 src2 ->
     isCorrectPC (WCap pc_p pc_b pc_e pc_a) →
-    regs !! PC = Some (WCap pc_p pc_b pc_e pc_a) →
-    regs_of (Subseg dst src1 src2) ⊆ dom _ regs →
+    regs !! (i, PC) = Some (WCap pc_p pc_b pc_e pc_a) →
+    regs_of_core (Subseg dst src1 src2) i ⊆ dom _ regs →
     
     {{{ ▷ pc_a ↦ₐ w ∗
         ▷ [∗ map] k↦y ∈ regs, k ↦ᵣ y }}}
-      Instr Executable @ Ep
+      (i, Instr Executable) @ Ep
     {{{ regs' retv, RET retv;
-        ⌜ Subseg_spec regs dst src1 src2 regs' retv ⌝ ∗
+        ⌜ Subseg_spec i regs dst src1 src2 regs' retv ⌝ ∗
         pc_a ↦ₐ w ∗
         [∗ map] k↦y ∈ regs', k ↦ᵣ y }}}.
   Proof.
@@ -83,22 +83,23 @@ Section cap_lang_rules.
     iModIntro. iSplitR. by iPureIntro; apply normal_always_head_reducible.
     iNext. iIntros (e2 σ2 efs Hpstep).
     apply prim_step_exec_inv in Hpstep as (-> & -> & (c & -> & Hstep)).
-    iSplitR; auto. eapply step_exec_inv in Hstep; eauto.
+    iSplitR; auto. eapply core_step_exec_inv in Hstep; eauto.
     unfold exec in Hstep; cbn in Hstep.
 
     specialize (indom_regs_incl _ _ _ Dregs Hregs) as Hri.
     unfold regs_of in Hri, Dregs.
-    destruct (Hri dst) as [wdst [H'dst Hdst]]. by set_solver+.
+    destruct (Hri i dst) as [wdst [H'dst Hdst]]. by set_solver+.
 
-    destruct (addr_of_argument regs src1) as [a1|] eqn:Ha1;
+    destruct (addr_of_argument regs i src1) as [a1|] eqn:Ha1;
       pose proof Ha1 as H'a1; cycle 1.
     { destruct src1 as [| r1] eqn:?; cbn in Ha1, Hstep.
       { rewrite Hdst Ha1 /= in Hstep.
         assert (c = Failed ∧ σ2 = (r, m)) as (-> & ->).
         { repeat case_match; inv Hstep; auto. }
         iFailWP "Hφ" Subseg_fail_src1_nonaddr. }
-      subst src1. destruct (Hri r1) as [r1v [Hr'1 Hr1]].
-        by unfold regs_of_argument; set_solver+.
+      subst src1. destruct (Hri i r1) as [r1v [Hr'1 Hr1]].
+      rewrite /regs_of_argument /regs_of_core /regs_of /regs_of_argument
+         ; set_solver+.
       rewrite /addr_of_argument /= Hr'1 in Ha1.
       assert (c = Failed ∧ σ2 = (r, m)) as (-> & ->).
       { destruct r1v ; simplify_pair_eq.
@@ -110,15 +111,16 @@ Section cap_lang_rules.
       all: iFailWP "Hφ" Subseg_fail_src1_nonaddr. }
     apply (addr_of_arg_mono _ r) in Ha1; auto. rewrite Ha1 /= in Hstep.
 
-    destruct (addr_of_argument regs src2) as [a2|] eqn:Ha2;
+    destruct (addr_of_argument regs i src2) as [a2|] eqn:Ha2;
       pose proof Ha2 as H'a2; cycle 1.
     { destruct src2 as [| r2] eqn:?; cbn in Ha2, Hstep.
       { rewrite Hdst Ha2 /= in Hstep.
         assert (c = Failed ∧ σ2 = (r, m)) as (-> & ->).
         { repeat case_match; inv Hstep; auto. }
         iFailWP "Hφ" Subseg_fail_src2_nonaddr. }
-      subst src2. destruct (Hri r2) as [r2v [Hr'2 Hr2]].
-        by unfold regs_of_argument; set_solver+.
+      subst src2. destruct (Hri i r2) as [r2v [Hr'2 Hr2]].
+      rewrite /regs_of_argument /regs_of_core /regs_of /regs_of_argument
+         ; set_solver+.
       rewrite /addr_of_argument /= Hr'2 in Ha2.
       assert (c = Failed ∧ σ2 = (r, m)) as (-> & ->).
       { destruct r2v ; simplify_pair_eq.
@@ -144,29 +146,29 @@ Section cap_lang_rules.
     destruct (isWithin a1 a2 b e) eqn:Hiw; cycle 1.
     { destruct p; try congruence; inv Hstep ; iFailWP "Hφ" Subseg_fail_not_iswithin. }
 
-    destruct (incrementPC (<[ dst := (WCap p a1 a2 a) ]> regs)) eqn:Hregs';
+    destruct (incrementPC (<[ (i, dst) := (WCap p a1 a2 a) ]> regs) i) eqn:Hregs';
       pose proof Hregs' as H'regs'; cycle 1.
-    { assert (incrementPC (<[ dst := (WCap p a1 a2 a) ]> r) = None) as HH.
+    { assert (incrementPC (<[ (i, dst) := (WCap p a1 a2 a) ]> r) i = None) as HH.
        { eapply incrementPC_overflow_mono; first eapply Hregs'.
          by rewrite lookup_insert_is_Some'; eauto.
          by apply insert_mono; eauto. }
-       apply (incrementPC_fail_updatePC _ m) in HH. rewrite HH in Hstep.
+       apply (incrementPC_fail_updatePC _ i m) in HH. rewrite HH in Hstep.
        assert (c = Failed ∧ σ2 = (r, m)) as (-> & ->)
            by (destruct p; inversion Hstep; auto).
        iFailWP "Hφ" Subseg_fail_incrPC. }
 
-    eapply (incrementPC_success_updatePC _ m) in Hregs'
+    eapply (incrementPC_success_updatePC _ i m) in Hregs'
       as (p' & g' & b' & e' & a'' & a_pc' & HPC'' & HuPC & ->).
     eapply updatePC_success_incl with (m':=m) in HuPC. 2: by eapply insert_mono; eauto. rewrite HuPC in Hstep.
      eassert ((c, σ2) = (NextI, _)) as HH.
      { destruct p; cbn in Hstep; eauto. congruence. }
     simplify_pair_eq. iFrame.
-    iMod ((gen_heap_update_inSepM _ _ dst) with "Hr Hmap") as "[Hr Hmap]"; eauto.
-    iMod ((gen_heap_update_inSepM _ _ PC) with "Hr Hmap") as "[Hr Hmap]"; eauto.
+    iMod ((gen_heap_update_inSepM _ _ (i, dst)) with "Hr Hmap") as "[Hr Hmap]"; eauto.
+    iMod ((gen_heap_update_inSepM _ _ (i, PC)) with "Hr Hmap") as "[Hr Hmap]"; eauto.
     iFrame. iApply "Hφ". iFrame. iPureIntro. econstructor; eauto.
   Qed.
 
-  Lemma wp_subseg_success E pc_p pc_b pc_e pc_a w dst r1 r2 p b e a n1 n2 a1 a2 pc_a' :
+  Lemma wp_subseg_success E i pc_p pc_b pc_e pc_a w dst r1 r2 p b e a n1 n2 a1 a2 pc_a' :
     decodeInstrW w = Subseg dst (inr r1) (inr r2) →
     isCorrectPC (WCap pc_p pc_b pc_e pc_a) →
     z_to_addr n1 = Some a1 → z_to_addr n2 = Some a2 →
@@ -174,39 +176,44 @@ Section cap_lang_rules.
     isWithin a1 a2 b e = true →
     (pc_a + 1)%a = Some pc_a' →
     
-    {{{ ▷ PC ↦ᵣ WCap pc_p pc_b pc_e pc_a
+    {{{ ▷ (i, PC) ↦ᵣ WCap pc_p pc_b pc_e pc_a
         ∗ ▷ pc_a ↦ₐ w
-        ∗ ▷ dst ↦ᵣ WCap p b e a
-        ∗ ▷ r1 ↦ᵣ WInt n1
-        ∗ ▷ r2 ↦ᵣ WInt n2 }}}
-      Instr Executable @ E
-      {{{ RET NextIV;
-          PC ↦ᵣ WCap pc_p pc_b pc_e pc_a'
+        ∗ ▷ (i, dst) ↦ᵣ WCap p b e a
+        ∗ ▷ (i, r1) ↦ᵣ WInt n1
+        ∗ ▷ (i, r2) ↦ᵣ WInt n2 }}}
+      (i, Instr Executable) @ E
+      {{{ RET (i, NextIV);
+          (i, PC) ↦ᵣ WCap pc_p pc_b pc_e pc_a'
           ∗ pc_a ↦ₐ w
-          ∗ r1 ↦ᵣ WInt n1
-          ∗ r2 ↦ᵣ WInt n2
-          ∗ dst ↦ᵣ WCap p a1 a2 a
+          ∗ (i, r1) ↦ᵣ WInt n1
+          ∗ (i, r2) ↦ᵣ WInt n2
+          ∗ (i, dst) ↦ᵣ WCap p a1 a2 a
       }}}.
   Proof.
     iIntros (Hinstr Hvpc Hn1 Hn2 Hpne Hwb Hpc_a' ϕ) "(>HPC & >Hpc_a & >Hdst & >Hr1 & >Hr2) Hφ".
     iDestruct (map_of_regs_4 with "HPC Hr1 Hr2 Hdst") as "[Hmap (%&%&%&%&%&%)]".
     iApply (wp_Subseg with "[$Hmap Hpc_a]"); eauto; simplify_map_eq; eauto.
-    by unfold regs_of; rewrite !dom_insert; set_solver+.
+    by unfold regs_of_core; rewrite !dom_insert; set_solver+.
     iNext. iIntros (regs' retv) "(#Hspec & Hpc_a & Hmap)". iDestruct "Hspec" as %Hspec.
 
     destruct Hspec as [| * Hfail].
     { (* Success *)
       iApply "Hφ". iFrame. incrementPC_inv; simplify_map_eq.
-      unfold addr_of_argument, z_of_argument in *. simplify_map_eq.
-      rewrite (insert_commute _ PC dst) // insert_insert (insert_commute _ r2 dst) //
-              (insert_commute _ r1 dst) // (insert_commute _ PC dst) // insert_insert.
+      unfold addr_of_argument, z_of_argument in *.
+      simplify_map_eq by simplify_pair_eq.
+      rewrite (insert_commute _ (i, PC) (i, dst)) ; simplify_pair_eq.
+      rewrite insert_insert (insert_commute _ (i, r2) (i, dst)) ; simplify_pair_eq.
+      rewrite (insert_commute _ (i, r1) (i, dst)) ; simplify_pair_eq.
+      rewrite (insert_commute _ (i, PC) (i, dst)) ; simplify_pair_eq.
+      rewrite insert_insert.
+
       iDestruct (regs_of_map_4 with "Hmap") as "(?&?&?&?)"; eauto; iFrame. }
     { (* Failure (contradiction) *)
       destruct Hfail; try incrementPC_inv; unfold addr_of_argument, z_of_argument in *.
-      all: simplify_map_eq; eauto; congruence. }
+      all: simplify_map_eq by simplify_pair_eq; eauto; congruence. }
   Qed.
 
-  Lemma wp_subseg_success_same E pc_p pc_b pc_e pc_a w dst r1 p b e a n1 a1 pc_a' :
+  Lemma wp_subseg_success_same E i pc_p pc_b pc_e pc_a w dst r1 p b e a n1 a1 pc_a' :
     decodeInstrW w = Subseg dst (inr r1) (inr r1) →
     isCorrectPC (WCap pc_p pc_b pc_e pc_a) →
     z_to_addr n1 = Some a1 →
@@ -214,37 +221,41 @@ Section cap_lang_rules.
     isWithin a1 a1 b e = true →
     (pc_a + 1)%a = Some pc_a' →
     
-    {{{ ▷ PC ↦ᵣ WCap pc_p pc_b pc_e pc_a
+    {{{ ▷ (i, PC) ↦ᵣ WCap pc_p pc_b pc_e pc_a
         ∗ ▷ pc_a ↦ₐ w
-        ∗ ▷ dst ↦ᵣ WCap p b e a
-        ∗ ▷ r1 ↦ᵣ WInt n1 }}}
-      Instr Executable @ E
-      {{{ RET NextIV;
-          PC ↦ᵣ WCap pc_p pc_b pc_e pc_a'
+        ∗ ▷ (i, dst) ↦ᵣ WCap p b e a
+        ∗ ▷ (i, r1) ↦ᵣ WInt n1 }}}
+      (i, Instr Executable) @ E
+      {{{ RET (i, NextIV);
+          (i, PC) ↦ᵣ WCap pc_p pc_b pc_e pc_a'
           ∗ pc_a ↦ₐ w
-          ∗ r1 ↦ᵣ WInt n1
-          ∗ dst ↦ᵣ WCap p a1 a1 a
+          ∗ (i, r1) ↦ᵣ WInt n1
+          ∗ (i, dst) ↦ᵣ WCap p a1 a1 a
       }}}.
   Proof.
     iIntros (Hinstr Hvpc Hn1 Hpne Hwb Hpc_a' ϕ) "(>HPC & >Hpc_a & >Hdst & >Hr1) Hφ".
     iDestruct (map_of_regs_3 with "HPC Hr1 Hdst") as "[Hmap (%&%&%)]".
-    iApply (wp_Subseg with "[$Hmap Hpc_a]"); eauto; simplify_map_eq; eauto.
-    by unfold regs_of; rewrite !dom_insert; set_solver+.
+    iApply (wp_Subseg with "[$Hmap Hpc_a]"); eauto; simplify_map_eq by simplify_pair_eq; eauto.
+    by unfold regs_of_core; rewrite !dom_insert; set_solver+.
     iNext. iIntros (regs' retv) "(#Hspec & Hpc_a & Hmap)". iDestruct "Hspec" as %Hspec.
 
     destruct Hspec as [| * Hfail].
     { (* Success *)
-      iApply "Hφ". iFrame. incrementPC_inv; simplify_map_eq.
-      unfold addr_of_argument, z_of_argument in *. simplify_map_eq.
-      rewrite (insert_commute _ PC dst) // insert_insert (insert_commute _ r1 dst) //
-              (insert_commute _ PC dst) // insert_insert.
+      iApply "Hφ". iFrame. incrementPC_inv; simplify_map_eq by simplify_pair_eq.
+      unfold addr_of_argument, z_of_argument in *.
+      simplify_map_eq by simplify_pair_eq.
+
+      rewrite (insert_commute _ (i, PC) (i, dst)) ; simplify_pair_eq.
+      rewrite insert_insert (insert_commute _ (i, r1) (i, dst)) ; simplify_pair_eq.
+      rewrite (insert_commute _ (i, PC) (i, dst)) ; simplify_pair_eq.
+      rewrite insert_insert.
       iDestruct (regs_of_map_3 with "Hmap") as "(?&?&?)"; eauto; iFrame. }
     { (* Failure (contradiction) *)
       destruct Hfail; try incrementPC_inv; unfold addr_of_argument, z_of_argument in *.
-      all: simplify_map_eq; eauto; congruence. }
+      all: simplify_map_eq by simplify_pair_eq; eauto; congruence. }
   Qed.
 
-  Lemma wp_subseg_success_l E pc_p pc_b pc_e pc_a w dst r2 p b e a n1 n2 a1 a2 pc_a' :
+  Lemma wp_subseg_success_l E i pc_p pc_b pc_e pc_a w dst r2 p b e a n1 n2 a1 a2 pc_a' :
     decodeInstrW w = Subseg dst (inl n1) (inr r2) →
     isCorrectPC (WCap pc_p pc_b pc_e pc_a) →
     z_to_addr n1 = Some a1 → z_to_addr n2 = Some a2 →
@@ -252,37 +263,40 @@ Section cap_lang_rules.
     isWithin a1 a2 b e = true →
     (pc_a + 1)%a = Some pc_a' →
     
-    {{{ ▷ PC ↦ᵣ WCap pc_p pc_b pc_e pc_a
+    {{{ ▷ (i, PC) ↦ᵣ WCap pc_p pc_b pc_e pc_a
         ∗ ▷ pc_a ↦ₐ w
-        ∗ ▷ dst ↦ᵣ WCap p b e a
-        ∗ ▷ r2 ↦ᵣ WInt n2 }}}
-      Instr Executable @ E
-      {{{ RET NextIV;
-          PC ↦ᵣ WCap pc_p pc_b pc_e pc_a'
+        ∗ ▷ (i, dst) ↦ᵣ WCap p b e a
+        ∗ ▷ (i, r2) ↦ᵣ WInt n2 }}}
+      (i, Instr Executable) @ E
+      {{{ RET (i, NextIV);
+          (i, PC) ↦ᵣ WCap pc_p pc_b pc_e pc_a'
           ∗ pc_a ↦ₐ w
-          ∗ r2 ↦ᵣ WInt n2
-          ∗ dst ↦ᵣ WCap p a1 a2 a
+          ∗ (i, r2) ↦ᵣ WInt n2
+          ∗ (i, dst) ↦ᵣ WCap p a1 a2 a
       }}}.
   Proof.
     iIntros (Hinstr Hvpc Hn1 Hn2 Hpne Hwb Hpc_a' ϕ) "(>HPC & >Hpc_a & >Hdst & >Hr2) Hφ".
     iDestruct (map_of_regs_3 with "HPC Hr2 Hdst") as "[Hmap (%&%&%)]".
-    iApply (wp_Subseg with "[$Hmap Hpc_a]"); eauto; simplify_map_eq; eauto.
-    by unfold regs_of; rewrite !dom_insert; set_solver+.
+    iApply (wp_Subseg with "[$Hmap Hpc_a]"); eauto; simplify_map_eq by simplify_pair_eq; eauto.
+    by unfold regs_of_core; rewrite !dom_insert; set_solver+.
     iNext. iIntros (regs' retv) "(#Hspec & Hpc_a & Hmap)". iDestruct "Hspec" as %Hspec.
 
     destruct Hspec as [| * Hfail].
     { (* Success *)
-      iApply "Hφ". iFrame. incrementPC_inv; simplify_map_eq.
-      unfold addr_of_argument, z_of_argument in *. simplify_map_eq.
-      rewrite (insert_commute _ PC dst) // insert_insert (insert_commute _ r2 dst) //
-              (insert_commute _ PC dst) // insert_insert.
+      iApply "Hφ". iFrame. incrementPC_inv; simplify_map_eq by simplify_pair_eq.
+      unfold addr_of_argument, z_of_argument in *.
+      simplify_map_eq by simplify_pair_eq.
+      rewrite (insert_commute _ (i, PC) (i, dst)) ; simplify_pair_eq.
+      rewrite insert_insert (insert_commute _ (i, r2) (i, dst)) ; simplify_pair_eq.
+      rewrite (insert_commute _ (i, PC) (i, dst)) ; simplify_pair_eq.
+      rewrite insert_insert.
       iDestruct (regs_of_map_3 with "Hmap") as "(?&?&?)"; eauto; iFrame. }
     { (* Failure (contradiction) *)
       destruct Hfail; try incrementPC_inv; unfold addr_of_argument, z_of_argument in *.
-      all: simplify_map_eq; eauto; congruence. }
+      all: simplify_map_eq by simplify_pair_eq; eauto; congruence. }
   Qed.
 
-  Lemma wp_subseg_success_r E pc_p pc_b pc_e pc_a w dst r1 p b e a n1 n2 a1 a2 pc_a' :
+  Lemma wp_subseg_success_r E i pc_p pc_b pc_e pc_a w dst r1 p b e a n1 n2 a1 a2 pc_a' :
     decodeInstrW w = Subseg dst (inr r1) (inl n2) →
     isCorrectPC (WCap pc_p pc_b pc_e pc_a) →
     z_to_addr n1 = Some a1 → z_to_addr n2 = Some a2 →
@@ -290,37 +304,40 @@ Section cap_lang_rules.
     isWithin a1 a2 b e = true →
     (pc_a + 1)%a = Some pc_a' →
     
-    {{{ ▷ PC ↦ᵣ WCap pc_p pc_b pc_e pc_a
+    {{{ ▷ (i, PC) ↦ᵣ WCap pc_p pc_b pc_e pc_a
         ∗ ▷ pc_a ↦ₐ w
-        ∗ ▷ dst ↦ᵣ WCap p b e a
-        ∗ ▷ r1 ↦ᵣ WInt n1 }}}
-      Instr Executable @ E
-      {{{ RET NextIV;
-          PC ↦ᵣ WCap pc_p pc_b pc_e pc_a'
+        ∗ ▷ (i, dst) ↦ᵣ WCap p b e a
+        ∗ ▷ (i, r1) ↦ᵣ WInt n1 }}}
+      (i, Instr Executable) @ E
+      {{{ RET (i, NextIV);
+          (i, PC) ↦ᵣ WCap pc_p pc_b pc_e pc_a'
           ∗ pc_a ↦ₐ w
-          ∗ r1 ↦ᵣ WInt n1
-          ∗ dst ↦ᵣ WCap p a1 a2 a
+          ∗ (i, r1) ↦ᵣ WInt n1
+          ∗ (i, dst) ↦ᵣ WCap p a1 a2 a
       }}}.
   Proof.
     iIntros (Hinstr Hvpc Hn1 Hn2 Hpne Hwb Hpc_a' ϕ) "(>HPC & >Hpc_a & >Hdst & >Hr1) Hφ".
     iDestruct (map_of_regs_3 with "HPC Hr1 Hdst") as "[Hmap (%&%&%)]".
-    iApply (wp_Subseg with "[$Hmap Hpc_a]"); eauto; simplify_map_eq; eauto.
-    by unfold regs_of; rewrite !dom_insert; set_solver+.
+    iApply (wp_Subseg with "[$Hmap Hpc_a]"); eauto; simplify_map_eq by simplify_pair_eq; eauto.
+    by unfold regs_of_core; rewrite !dom_insert; set_solver+.
     iNext. iIntros (regs' retv) "(#Hspec & Hpc_a & Hmap)". iDestruct "Hspec" as %Hspec.
 
     destruct Hspec as [| * Hfail].
     { (* Success *)
-      iApply "Hφ". iFrame. incrementPC_inv; simplify_map_eq.
-      unfold addr_of_argument, z_of_argument in *. simplify_map_eq.
-      rewrite (insert_commute _ PC dst) // insert_insert (insert_commute _ r1 dst) //
-              (insert_commute _ PC dst) // insert_insert.
+      iApply "Hφ". iFrame. incrementPC_inv; simplify_map_eq by simplify_pair_eq.
+      unfold addr_of_argument, z_of_argument in *. simplify_map_eq
+        by simplify_pair_eq.
+      rewrite (insert_commute _ (i, PC) (i, dst)) ; simplify_pair_eq.
+      rewrite insert_insert (insert_commute _ (i, r1) (i, dst)) ; simplify_pair_eq.
+      rewrite (insert_commute _ (i, PC) (i, dst)) ; simplify_pair_eq.
+      rewrite insert_insert.
       iDestruct (regs_of_map_3 with "Hmap") as "(?&?&?)"; eauto; iFrame. }
     { (* Failure (contradiction) *)
       destruct Hfail; try incrementPC_inv; unfold addr_of_argument, z_of_argument in *.
-      all: simplify_map_eq; eauto; congruence. }
+      all: simplify_map_eq by simplify_pair_eq; eauto; congruence. }
   Qed.
 
-  Lemma wp_subseg_success_lr E pc_p pc_b pc_e pc_a w dst p b e a n1 n2 a1 a2 pc_a' :
+  Lemma wp_subseg_success_lr E i pc_p pc_b pc_e pc_a w dst p b e a n1 n2 a1 a2 pc_a' :
     decodeInstrW w = Subseg dst (inl n1) (inl n2) →
     isCorrectPC (WCap pc_p pc_b pc_e pc_a) →
     z_to_addr n1 = Some a1 → z_to_addr n2 = Some a2 →
@@ -328,34 +345,36 @@ Section cap_lang_rules.
     isWithin a1 a2 b e = true →
     (pc_a + 1)%a = Some pc_a' →
     
-    {{{ ▷ PC ↦ᵣ WCap pc_p pc_b pc_e pc_a
+    {{{ ▷ (i, PC) ↦ᵣ WCap pc_p pc_b pc_e pc_a
         ∗ ▷ pc_a ↦ₐ w
-        ∗ ▷ dst ↦ᵣ WCap p b e a }}}
-      Instr Executable @ E
-      {{{ RET NextIV;
-          PC ↦ᵣ WCap pc_p pc_b pc_e pc_a'
+        ∗ ▷ (i, dst) ↦ᵣ WCap p b e a }}}
+      (i, Instr Executable) @ E
+      {{{ RET (i, NextIV);
+          (i, PC) ↦ᵣ WCap pc_p pc_b pc_e pc_a'
           ∗ pc_a ↦ₐ w
-          ∗ dst ↦ᵣ WCap p a1 a2 a
+          ∗ (i, dst) ↦ᵣ WCap p a1 a2 a
       }}}.
   Proof.
     iIntros (Hinstr Hvpc Hn1 Hn2 Hpne Hwb Hpc_a' ϕ) "(>HPC & >Hpc_a & >Hdst) Hφ".
     iDestruct (map_of_regs_2 with "HPC Hdst") as "[Hmap %]".
-    iApply (wp_Subseg with "[$Hmap Hpc_a]"); eauto; simplify_map_eq; eauto.
+    iApply (wp_Subseg with "[$Hmap Hpc_a]"); eauto; simplify_map_eq by simplify_pair_eq; eauto.
     by unfold regs_of; rewrite !dom_insert; set_solver+.
     iNext. iIntros (regs' retv) "(#Hspec & Hpc_a & Hmap)". iDestruct "Hspec" as %Hspec.
 
     destruct Hspec as [| * Hfail].
     { (* Success *)
-      iApply "Hφ". iFrame. incrementPC_inv; simplify_map_eq.
-      unfold addr_of_argument, z_of_argument in *. simplify_map_eq.
-      rewrite (insert_commute _ PC dst) // insert_insert insert_commute // insert_insert.
+      iApply "Hφ". iFrame. incrementPC_inv; simplify_map_eq by simplify_pair_eq.
+      unfold addr_of_argument, z_of_argument in *. simplify_map_eq by simplify_pair_eq.
+      rewrite (insert_commute _ (i, PC) (i, dst)) ; simplify_pair_eq.
+      rewrite insert_insert insert_commute ; simplify_pair_eq.
+      rewrite insert_insert.
       iDestruct (regs_of_map_2 with "Hmap") as "(?&?)"; eauto; iFrame. }
     { (* Failure (contradiction) *)
       destruct Hfail; try incrementPC_inv; unfold addr_of_argument, z_of_argument in *.
-      all: simplify_map_eq; eauto; congruence. }
+      all: simplify_map_eq by simplify_pair_eq; eauto; congruence. }
   Qed.
 
-  Lemma wp_subseg_success_pc E pc_p pc_b pc_e pc_a w r1 r2 n1 n2 a1 a2 pc_a' :
+  Lemma wp_subseg_success_pc E i pc_p pc_b pc_e pc_a w r1 r2 n1 n2 a1 a2 pc_a' :
     decodeInstrW w = Subseg PC (inr r1) (inr r2) →
     isCorrectPC (WCap pc_p pc_b pc_e pc_a) →
     z_to_addr n1 = Some a1 → z_to_addr n2 = Some a2 →
@@ -363,36 +382,36 @@ Section cap_lang_rules.
     isWithin a1 a2 pc_b pc_e = true →
     (pc_a + 1)%a = Some pc_a' →
     
-    {{{ ▷ PC ↦ᵣ WCap pc_p pc_b pc_e pc_a
+    {{{ ▷ (i, PC) ↦ᵣ WCap pc_p pc_b pc_e pc_a
         ∗ ▷ pc_a ↦ₐ w
-        ∗ ▷ r1 ↦ᵣ WInt n1
-        ∗ ▷ r2 ↦ᵣ WInt n2 }}}
-      Instr Executable @ E
-      {{{ RET NextIV;
-          PC ↦ᵣ WCap pc_p a1 a2 pc_a'
+        ∗ ▷ (i, r1) ↦ᵣ WInt n1
+        ∗ ▷ (i, r2) ↦ᵣ WInt n2 }}}
+      (i, Instr Executable) @ E
+      {{{ RET (i, NextIV);
+          (i, PC) ↦ᵣ WCap pc_p a1 a2 pc_a'
           ∗ pc_a ↦ₐ w
-          ∗ r1 ↦ᵣ WInt n1
-          ∗ r2 ↦ᵣ WInt n2
+          ∗ (i, r1) ↦ᵣ WInt n1
+          ∗ (i, r2) ↦ᵣ WInt n2
       }}}.
   Proof.
     iIntros (Hinstr Hvpc Hn1 Hn2 Hpne Hwb Hpc_a' ϕ) "(>HPC & >Hpc_a & >Hr1 & >Hr2) Hφ".
     iDestruct (map_of_regs_3 with "HPC Hr1 Hr2") as "[Hmap (%&%&%)]".
-    iApply (wp_Subseg with "[$Hmap Hpc_a]"); eauto; simplify_map_eq; eauto.
-    by unfold regs_of; rewrite !dom_insert; set_solver+.
+    iApply (wp_Subseg with "[$Hmap Hpc_a]"); eauto; simplify_map_eq by simplify_pair_eq; eauto.
+    by unfold regs_of_core; rewrite !dom_insert; set_solver+.
     iNext. iIntros (regs' retv) "(#Hspec & Hpc_a & Hmap)". iDestruct "Hspec" as %Hspec.
 
     destruct Hspec as [| * Hfail].
     { (* Success *)
-      iApply "Hφ". iFrame. incrementPC_inv; simplify_map_eq.
-      unfold addr_of_argument, z_of_argument in *. simplify_map_eq.
+      iApply "Hφ". iFrame. incrementPC_inv; simplify_map_eq by simplify_pair_eq.
+      unfold addr_of_argument, z_of_argument in *. simplify_map_eq by simplify_pair_eq.
       rewrite !insert_insert.
       iDestruct (regs_of_map_3 with "Hmap") as "(?&?&?)"; eauto; iFrame. }
     { (* Failure (contradiction) *)
       destruct Hfail; try incrementPC_inv; unfold addr_of_argument, z_of_argument in *.
-      all: simplify_map_eq; eauto; try congruence. congruence. }
+      all: simplify_map_eq by simplify_pair_eq; eauto; try congruence. congruence. }
   Qed.
 
-  Lemma wp_subseg_success_pc_same E pc_p pc_b pc_e pc_a w r1 n1 a1 pc_a' :
+  Lemma wp_subseg_success_pc_same E i pc_p pc_b pc_e pc_a w r1 n1 a1 pc_a' :
     decodeInstrW w = Subseg PC (inr r1) (inr r1) →
     isCorrectPC (WCap pc_p pc_b pc_e pc_a) →
     z_to_addr n1 = Some a1 →
@@ -400,34 +419,36 @@ Section cap_lang_rules.
     isWithin a1 a1 pc_b pc_e = true →
     (pc_a + 1)%a = Some pc_a' →
     
-    {{{ ▷ PC ↦ᵣ WCap pc_p pc_b pc_e pc_a
+    {{{ ▷ (i, PC) ↦ᵣ WCap pc_p pc_b pc_e pc_a
         ∗ ▷ pc_a ↦ₐ w
-        ∗ ▷ r1 ↦ᵣ WInt n1 }}}
-      Instr Executable @ E
-      {{{ RET NextIV;
-          PC ↦ᵣ WCap pc_p a1 a1 pc_a'
+        ∗ ▷ (i, r1) ↦ᵣ WInt n1 }}}
+      (i, Instr Executable) @ E
+      {{{ RET (i, NextIV);
+          (i, PC) ↦ᵣ WCap pc_p a1 a1 pc_a'
           ∗ pc_a ↦ₐ w
-          ∗ r1 ↦ᵣ WInt n1
+          ∗ (i, r1) ↦ᵣ WInt n1
       }}}.
   Proof.
     iIntros (Hinstr Hvpc Hn1 Hpne Hwb Hpc_a' ϕ) "(>HPC & >Hpc_a & >Hr1) Hφ".
     iDestruct (map_of_regs_2 with "HPC Hr1") as "[Hmap %]".
-    iApply (wp_Subseg with "[$Hmap Hpc_a]"); eauto; simplify_map_eq; eauto.
-    by unfold regs_of; rewrite !dom_insert; set_solver+.
+    iApply (wp_Subseg with "[$Hmap Hpc_a]"); eauto; simplify_map_eq by simplify_pair_eq; eauto.
+    by unfold regs_of_core; rewrite !dom_insert; set_solver+.
     iNext. iIntros (regs' retv) "(#Hspec & Hpc_a & Hmap)". iDestruct "Hspec" as %Hspec.
 
     destruct Hspec as [| * Hfail].
     { (* Success *)
-      iApply "Hφ". iFrame. incrementPC_inv; simplify_map_eq.
-      unfold addr_of_argument, z_of_argument in *. simplify_map_eq.
-      rewrite (insert_commute _ PC r1) // insert_insert insert_commute // insert_insert.
+      iApply "Hφ". iFrame. incrementPC_inv; simplify_map_eq by simplify_pair_eq.
+      unfold addr_of_argument, z_of_argument in *. simplify_map_eq by simplify_pair_eq.
+      rewrite (insert_commute _ (i, PC) (i, r1)) ; simplify_pair_eq.
+      rewrite insert_insert insert_commute ; simplify_pair_eq.
+      rewrite insert_insert.
       iDestruct (regs_of_map_2 with "Hmap") as "(?&?)"; eauto; iFrame. }
     { (* Failure (contradiction) *)
       destruct Hfail; try incrementPC_inv; unfold addr_of_argument, z_of_argument in *.
-      all: simplify_map_eq; eauto; try congruence. congruence. }
+      all: simplify_map_eq by simplify_pair_eq; eauto; try congruence. congruence. }
   Qed.
 
-  Lemma wp_subseg_success_pc_l E pc_p pc_b pc_e pc_a w r2 n1 n2 a1 a2 pc_a' :
+  Lemma wp_subseg_success_pc_l E i pc_p pc_b pc_e pc_a w r2 n1 n2 a1 a2 pc_a' :
     decodeInstrW w = Subseg PC (inl n1) (inr r2) →
     isCorrectPC (WCap pc_p pc_b pc_e pc_a) →
     z_to_addr n1 = Some a1 → z_to_addr n2 = Some a2 →
@@ -435,34 +456,37 @@ Section cap_lang_rules.
     isWithin a1 a2 pc_b pc_e = true →
     (pc_a + 1)%a = Some pc_a' →
     
-    {{{ ▷ PC ↦ᵣ WCap pc_p pc_b pc_e pc_a
+    {{{ ▷ (i, PC) ↦ᵣ WCap pc_p pc_b pc_e pc_a
         ∗ ▷ pc_a ↦ₐ w
-        ∗ ▷ r2 ↦ᵣ WInt n2 }}}
-      Instr Executable @ E
-      {{{ RET NextIV;
-          PC ↦ᵣ WCap pc_p a1 a2 pc_a'
+        ∗ ▷ (i, r2) ↦ᵣ WInt n2 }}}
+      (i, Instr Executable) @ E
+      {{{ RET (i, NextIV);
+          (i, PC) ↦ᵣ WCap pc_p a1 a2 pc_a'
           ∗ pc_a ↦ₐ w
-          ∗ r2 ↦ᵣ WInt n2
+          ∗ (i, r2) ↦ᵣ WInt n2
       }}}.
   Proof.
     iIntros (Hinstr Hvpc Hn1 Hn2 Hpne Hwb Hpc_a' ϕ) "(>HPC & >Hpc_a & >Hr2) Hφ".
     iDestruct (map_of_regs_2 with "HPC Hr2") as "[Hmap %]".
-    iApply (wp_Subseg with "[$Hmap Hpc_a]"); eauto; simplify_map_eq; eauto.
-    by unfold regs_of; rewrite !dom_insert; set_solver+.
+    iApply (wp_Subseg with "[$Hmap Hpc_a]"); eauto; simplify_map_eq by simplify_pair_eq; eauto.
+    by unfold regs_of_core; rewrite !dom_insert; set_solver+.
     iNext. iIntros (regs' retv) "(#Hspec & Hpc_a & Hmap)". iDestruct "Hspec" as %Hspec.
 
     destruct Hspec as [| * Hfail].
     { (* Success *)
-      iApply "Hφ". iFrame. incrementPC_inv; simplify_map_eq.
-      unfold addr_of_argument, z_of_argument in *. simplify_map_eq.
-      rewrite (insert_commute _ PC r2) // insert_insert insert_commute // insert_insert.
+      iApply "Hφ". iFrame. incrementPC_inv; simplify_map_eq by simplify_pair_eq.
+      unfold addr_of_argument, z_of_argument in *. simplify_map_eq
+        by simplify_pair_eq.
+      rewrite (insert_commute _ (i, PC) (i, r2)) ; simplify_pair_eq.
+      rewrite insert_insert insert_commute ; simplify_pair_eq.
+      rewrite insert_insert.
       iDestruct (regs_of_map_2 with "Hmap") as "(?&?)"; eauto; iFrame. }
     { (* Failure (contradiction) *)
       destruct Hfail; try incrementPC_inv; unfold addr_of_argument, z_of_argument in *.
-      all: simplify_map_eq; eauto; try congruence. congruence. }
+      all: simplify_map_eq by simplify_pair_eq; eauto; try congruence. congruence. }
   Qed.
 
-  Lemma wp_subseg_success_pc_r E pc_p pc_b pc_e pc_a w r1 n1 n2 a1 a2 pc_a' :
+  Lemma wp_subseg_success_pc_r E i pc_p pc_b pc_e pc_a w r1 n1 n2 a1 a2 pc_a' :
     decodeInstrW w = Subseg PC (inr r1) (inl n2) →
     isCorrectPC (WCap pc_p pc_b pc_e pc_a) →
     z_to_addr n1 = Some a1 → z_to_addr n2 = Some a2 →
@@ -470,34 +494,37 @@ Section cap_lang_rules.
     isWithin a1 a2 pc_b pc_e = true →
     (pc_a + 1)%a = Some pc_a' →
     
-    {{{ ▷ PC ↦ᵣ WCap pc_p pc_b pc_e pc_a
+    {{{ ▷ (i, PC) ↦ᵣ WCap pc_p pc_b pc_e pc_a
         ∗ ▷ pc_a ↦ₐ w
-        ∗ ▷ r1 ↦ᵣ WInt n1 }}}
-      Instr Executable @ E
-      {{{ RET NextIV;
-          PC ↦ᵣ WCap pc_p a1 a2 pc_a'
+        ∗ ▷ (i, r1) ↦ᵣ WInt n1 }}}
+      (i, Instr Executable) @ E
+      {{{ RET (i, NextIV);
+          (i, PC) ↦ᵣ WCap pc_p a1 a2 pc_a'
           ∗ pc_a ↦ₐ w
-          ∗ r1 ↦ᵣ WInt n1
+          ∗ (i, r1) ↦ᵣ WInt n1
       }}}.
   Proof.
     iIntros (Hinstr Hvpc Hn1 Hn2 Hpne Hwb Hpc_a' ϕ) "(>HPC & >Hpc_a & >Hr1) Hφ".
     iDestruct (map_of_regs_2 with "HPC Hr1") as "[Hmap %]".
-    iApply (wp_Subseg with "[$Hmap Hpc_a]"); eauto; simplify_map_eq; eauto.
-    by unfold regs_of; rewrite !dom_insert; set_solver+.
+    iApply (wp_Subseg with "[$Hmap Hpc_a]"); eauto; simplify_map_eq by simplify_pair_eq; eauto.
+    by unfold regs_of_core; rewrite !dom_insert; set_solver+.
     iNext. iIntros (regs' retv) "(#Hspec & Hpc_a & Hmap)". iDestruct "Hspec" as %Hspec.
 
     destruct Hspec as [| * Hfail].
     { (* Success *)
-      iApply "Hφ". iFrame. incrementPC_inv; simplify_map_eq.
-      unfold addr_of_argument, z_of_argument in *. simplify_map_eq.
-      rewrite (insert_commute _ PC r1) // insert_insert insert_commute // insert_insert.
+      iApply "Hφ". iFrame. incrementPC_inv; simplify_map_eq by simplify_pair_eq.
+      unfold addr_of_argument, z_of_argument in *.
+      simplify_map_eq by simplify_pair_eq.
+      rewrite (insert_commute _ (i, PC) (i, r1)) ; simplify_pair_eq.
+      rewrite insert_insert insert_commute ; simplify_pair_eq.
+      rewrite insert_insert.
       iDestruct (regs_of_map_2 with "Hmap") as "(?&?)"; eauto; iFrame. }
     { (* Failure (contradiction) *)
       destruct Hfail; try incrementPC_inv; unfold addr_of_argument, z_of_argument in *.
-      all: simplify_map_eq; eauto; try congruence. congruence. }
+      all: simplify_map_eq by simplify_pair_eq; eauto; try congruence. congruence. }
   Qed.
 
-  Lemma wp_subseg_success_pc_lr E pc_p pc_b pc_e pc_a w n1 n2 a1 a2 pc_a' :
+  Lemma wp_subseg_success_pc_lr E i pc_p pc_b pc_e pc_a w n1 n2 a1 a2 pc_a' :
     decodeInstrW w = Subseg PC (inl n1) (inl n2) →
     isCorrectPC (WCap pc_p pc_b pc_e pc_a) →
     z_to_addr n1 = Some a1 → z_to_addr n2 = Some a2 →
@@ -505,29 +532,29 @@ Section cap_lang_rules.
     isWithin a1 a2 pc_b pc_e = true →
     (pc_a + 1)%a = Some pc_a' →
     
-    {{{ ▷ PC ↦ᵣ WCap pc_p pc_b pc_e pc_a
+    {{{ ▷ (i, PC) ↦ᵣ WCap pc_p pc_b pc_e pc_a
         ∗ ▷ pc_a ↦ₐ w }}}
-      Instr Executable @ E
-      {{{ RET NextIV;
-          PC ↦ᵣ WCap pc_p a1 a2 pc_a'
+      (i, Instr Executable) @ E
+      {{{ RET (i, NextIV);
+          (i, PC) ↦ᵣ WCap pc_p a1 a2 pc_a'
           ∗ pc_a ↦ₐ w
       }}}.
   Proof.
     iIntros (Hinstr Hvpc Hn1 Hn2 Hpne Hwb Hpc_a' ϕ) "(>HPC & >Hpc_a) Hφ".
     iDestruct (map_of_regs_1 with "HPC") as "Hmap".
-    iApply (wp_Subseg with "[$Hmap Hpc_a]"); eauto; simplify_map_eq; eauto.
-    by unfold regs_of; rewrite !dom_insert; set_solver+.
+    iApply (wp_Subseg with "[$Hmap Hpc_a]"); eauto; simplify_map_eq by simplify_pair_eq; eauto.
+    by unfold regs_of_core; rewrite !dom_insert; set_solver+.
     iNext. iIntros (regs' retv) "(#Hspec & Hpc_a & Hmap)". iDestruct "Hspec" as %Hspec.
 
     destruct Hspec as [| * Hfail].
     { (* Success *)
-      iApply "Hφ". iFrame. incrementPC_inv; simplify_map_eq.
-      unfold addr_of_argument, z_of_argument in *. simplify_map_eq.
+      iApply "Hφ". iFrame. incrementPC_inv; simplify_map_eq by simplify_pair_eq.
+      unfold addr_of_argument, z_of_argument in *. simplify_map_eq by simplify_pair_eq.
       rewrite !insert_insert.
       iDestruct (regs_of_map_1 with "Hmap") as "?"; eauto; iFrame. }
     { (* Failure (contradiction) *)
       destruct Hfail; try incrementPC_inv; unfold addr_of_argument, z_of_argument in *.
-      all: simplify_map_eq; eauto; try congruence. congruence. }
+      all: simplify_map_eq by simplify_pair_eq; eauto; try congruence. congruence. }
   Qed.
 
 End cap_lang_rules.
